Refactoring the safety part

Compat.v
@@ -7,7 +7,7 @@ From Elo Require Import Access.
 
 Definition compat m m' t := forall ad,
   access m t ad ->
-  getTM m ad = getTM m' ad.
+  m[ad] = m'[ad].
 
 Lemma compat_refl : forall m t, 
   compat m m t.
@@ -24,7 +24,7 @@ Proof.
   try solve [symmetry; eauto using access].
   eapply IHHacc. intros ? ?.
   eapply Hcompat. eapply access_mem.
-  rewrite (Hcompat _ (access_loc _ _)).
+  rewrite (Hcompat _ (access_ref _ _ _)).
   trivial.
 Qed.
 
@@ -36,7 +36,7 @@ Proof.
   intros * Hcompat Hacc. unfold compat in *.
   induction Hacc; eauto using access.
   eapply access_mem.
-  rewrite <- (Hcompat _ (access_loc _ _)).
+  rewrite <- (Hcompat _ (access_ref _ _ _)).
   eapply IHHacc. intros ? ?.
   eapply Hcompat. eauto using access.
 Qed.
@@ -59,36 +59,36 @@ Qed.
 Lemma compat_inaccessible_address_set : forall m m' t ad v,
   compat m m' t ->
   ~ access m t ad ->
-  compat m (set m' ad v) t.
+  compat m m'[ad <- v] t.
 Proof.
   intros * Hcompat Hnacc ad Hacc. unfold compat in *.
-  induction Hacc; try solve [inversion_not_access; eauto using access].
+  induction Hacc; try solve [inversion_not_access Hnacc].
   match goal with H : ~ access _ _ ?ad' |- _ => 
     destruct (Nat.eq_dec ad ad'); subst
   end.
   - exfalso. eauto using access.
-  - rewrite (get_set_neq TM_Unit); eauto using access.
+  - rewrite_array TM_Unit. eauto using access.
 Qed.
 
 Lemma compat_inaccessible_address_add : forall m m' t v,
   compat m m' t ->
   ~ access m t (length m') ->
-  compat m (add m' v) t.
+  compat m (m' +++ v) t.
 Proof.
   intros * Hcompat Hnacc ad Hacc. unfold compat in *.
-  induction Hacc; try solve [inversion_not_access; eauto using access].
+  induction Hacc; try solve [inversion_not_access Hnacc; eauto using access].
   destruct (Nat.eq_dec ad (length m')); subst.
-  + exfalso. eauto using access.
-  + destruct (not_eq ad (length m')); trivial.
-    * rewrite (get_add_lt TM_Unit); eauto using access.
-    * specialize (Hcompat ad (access_loc m ad)).
-      rewrite (get_default TM_Unit m') in Hcompat; try lia.
-      rewrite (get_add_gt TM_Unit); trivial.
+  - exfalso. eauto using access.
+  - destruct (not_eq ad (length m')); trivial.
+    + rewrite_array TM_Unit. eauto using access.
+    + specialize (Hcompat ad (access_ref _ _ _)).
+      rewrite_array TM_Unit. rewrite (get_default TM_Unit m') in Hcompat;
+      trivial; lia.
 Qed.
 
 Corollary inaccessible_address_set_1 : forall m t ad ad' v,
   ~ access m t ad' ->
-  access (set m ad' v) t ad ->
+  access m[ad' <- v] t ad ->
   access m t ad.
 Proof.
   intros.
@@ -99,7 +99,7 @@ Qed.
 Corollary inaccessible_address_set_2  : forall m t ad ad' v,
   ~ access m t ad' ->
   ~ access m t ad ->
-  ~ access (set m ad' v) t ad.
+  ~ access m[ad' <- v] t ad.
 Proof.
   intros.
   eauto using compat_refl, compat_access_not, compat_inaccessible_address_set.
@@ -107,7 +107,7 @@ Qed.
 
 Corollary inaccessible_address_add_1 : forall m t ad v,
   ~ access m t (length m) ->
-  access (add m v) t ad ->
+  access (m +++ v) t ad ->
   access m t ad.
 Proof.
   intros.
@@ -118,7 +118,7 @@ Qed.
 Corollary inaccessible_address_add_2 : forall m t ad v,
   ~ access m t (length m) ->
   ~ access m t ad ->
-  ~ access (add m v) t ad.
+  ~ access (m +++ v) t ad.
 Proof.
   intros.
   eauto using compat_refl, compat_access_not, compat_inaccessible_address_add.
